chore: broken version\

RISCV/Instructions.lean
@@ -63,4 +63,7 @@ def srli (shamt : BitVec 6) (rs1_val : BitVec 64) : BitVec 64 := rs1_val >>> sha
   Performs arithmetic right shift on the value in register rs1 by the shift amount held in the
   lower 5 bits of the immediate In RV64, bit-25 is used to shamt[5].
 -/
-def srai (shamt : BitVec 6) (rs1_val : BitVec 64): BitVec 64 := BitVec.sshiftRight' rs1_val  shamt
+def srai (shamt : BitVec 6) (rs1_val : BitVec 64): BitVec 64 :=
+  let value := rs1_val
+  let shift := shamt.toNat
+  BitVec.setWidth 64 (BitVec.extractLsb (63 + shift) shift (BitVec.signExtend (64 + shift) value))
